Flatten the view record a bit

src/lib/views/Kuiper.IView.fsti
@@ -14,21 +14,9 @@ module SZ = Kuiper.SizeT
 [@@erasable]
 noeq
 inline_for_extraction noextract
-type aiview_schema = {
-  (* abstract index type *)
-  ait      : Type0;
-}
-
-[@@erasable]
-noeq
-inline_for_extraction noextract
 type aiview_step (from_ait to_ait : Type0) = {
   (* Index translation *)
   imap : from_ait @~> to_ait;
-}
-
-let raw_aiview_schema (len : nat) : aiview_schema = {
-  ait      = natlt len;
 }
 
 [@@erasable]
@@ -36,8 +24,8 @@ noeq
 inline_for_extraction noextract
 type aiview = {
   len  : nat;
-  sch  : aiview_schema;
-  step : aiview_step sch.ait (natlt len);
+  ait  : Type0;
+  step : aiview_step ait (natlt len);
 }
 
 unfold
@@ -57,21 +45,21 @@ let is_full_view_lempat (avw : aiview { is_full_view avw })
 // Can't really give this an SMT pattern...
 val full_iff_cardinal
   (vw : aiview)
-  {| Enumerable.enumerable vw.sch.ait |}
-  : Lemma (is_full_view vw <==> Enumerable.cardinal vw.sch.ait #_ == vw.len)
+  {| Enumerable.enumerable vw.ait |}
+  : Lemma (is_full_view vw <==> Enumerable.cardinal vw.ait #_ == vw.len)
 
 (* Nothing fancy here. *)
 inline_for_extraction noextract
 let raw_view (#len : erased nat) : aiview = {
   len  = len;
-  sch  = raw_aiview_schema len;
+  ait  = natlt len;
   step = { imap = inj_id; };
 }
 
 [@@erasable]
 noeq
 inline_for_extraction noextract
-type ciview_schema (asch : aiview_schema) = {
+type ciview_schema (ait : Type0) = {
   (* The concrete index type *)
   [@@@no_method]
   cit   : Type0;
@@ -80,11 +68,11 @@ type ciview_schema (asch : aiview_schema) = {
      Need not be executable. NOTE: Do not mark this erased, this
      worsens SMT performance significantly. This is already an erasable type. *)
   [@@@no_method]
-  bij   : asch.ait =~ cit;
+  bij   : ait =~ cit;
 }
 
 inline_for_extraction noextract
-let raw_ciview_schema (len : erased nat{SZ.fits len}) : ciview_schema (raw_aiview_schema len) = {
+let raw_ciview_schema (len : erased nat{SZ.fits len}) : ciview_schema (natlt len) = {
   cit = szlt len;
   bij = fin_size_t_bij _;
 }
@@ -93,10 +81,10 @@ let raw_ciview_schema (len : erased nat{SZ.fits len}) : ciview_schema (raw_aivie
 
 inline_for_extraction noextract
 class ciview_step
-  (#asch1 #asch2 : aiview_schema)
-  (csch1 : ciview_schema asch1)
-  (csch2 : ciview_schema asch2)
-  (step  : aiview_step asch1.ait asch2.ait)
+  (#ait1 #ait2 : Type0)
+  (csch1 : ciview_schema ait1)
+  (csch2 : ciview_schema ait2)
+  (step  : aiview_step ait1 ait2)
 =
 {
   (* Concrete index translation *)
@@ -115,7 +103,7 @@ class ciview_step
    *)
   [@@@no_method]
   compat :
-    ai : asch1.ait ->
+    ai : ait1 ->
       squash (cimap.cf (csch1.bij.ff ai) == csch2.bij.ff (step.imap.f ai));
 }
 
@@ -127,7 +115,7 @@ class ciview (avw : aiview) =
   clen : (clen : SZ.t {SZ.v clen == avw.len});
 
   [@@@no_method]
-  sch  : ciview_schema avw.sch;
+  sch  : ciview_schema avw.ait;
 
   [@@@no_method]
   step : ciview_step sch (raw_ciview_schema avw.len) avw.step;
@@ -158,12 +146,10 @@ let inj_bij' (#a #b : Type) (bij : a =~ b) : (b @~> a) =
 let reindex_view
   (vw : aiview)
   (#ait' : Type)
-  (bij : vw.sch.ait =~ ait')
+  (bij : vw.ait =~ ait')
   : aiview = {
   len = vw.len;
-  sch = {
-    ait      = ait';
-  };
+  ait = ait';
 
   step = {
     imap = inj_bij' bij `inj_comp` vw.step.imap;
@@ -172,17 +158,17 @@ let reindex_view
 
 let it_to_nat
   (vw : aiview)
-  (i : vw.sch.ait)
+  (i : vw.ait)
   : GTot (natlt vw.len)
   = i |~> vw.step.imap
 
 let it_of_nat
   (vw : aiview)
   (i: natlt vw.len{FStar.Functions.in_image vw.step.imap.f i})
-  : GTot vw.sch.ait
+  : GTot vw.ait
   = i <~| vw.step.imap
 
-val it_nat_rel (vw : aiview) (i : vw.sch.ait)
+val it_nat_rel (vw : aiview) (i : vw.ait)
   (j : natlt vw.len{FStar.Functions.in_image vw.step.imap.f j})
   : Lemma (it_to_nat vw i == j <==> i == it_of_nat vw j)
           [SMTPat (it_to_nat vw i); SMTPat (it_of_nat vw j)]
@@ -190,13 +176,13 @@ val it_nat_rel (vw : aiview) (i : vw.sch.ait)
 let ci_to_ai
   (vw : aiview) {| cw : ciview vw |}
   (i : cw.sch.cit)
-  : GTot vw.sch.ait
+  : GTot vw.ait
   = let open Kuiper.Bijection in
     i <~| cw.sch.bij
 
 let ai_to_ci
   (vw : aiview) {| cw : ciview vw |}
-  (i : vw.sch.ait)
+  (i : vw.ait)
   : GTot cw.sch.cit
   = let open Kuiper.Bijection in
     i |~> cw.sch.bij
@@ -206,9 +192,7 @@ let sum_aiview
   (#_ : squash (no_overlap vw1.step.imap.f vw2.step.imap.f))
   : aiview = {
   len = max vw1.len vw2.len;
-  sch = {
-    ait      = either vw1.sch.ait vw2.sch.ait;
-  };
+  ait = either vw1.ait vw2.ait;
   step = {
     imap     = {
       f      = merge_either vw1.step.imap.f vw2.step.imap.f;
@@ -226,12 +210,12 @@ let compose_astep (#sch1 #sch2 #sch3 : Type0)
 
 inline_for_extraction noextract
 let compose_cstep
-  (#asch1 #asch2 #asch3 : aiview_schema)
-  (#csch1 : ciview_schema asch1)
-  (#csch2 : ciview_schema asch2)
-  (#csch3 : ciview_schema asch3)
-  (#step12 : aiview_step asch1.ait asch2.ait)
-  (#step23 : aiview_step asch2.ait asch3.ait)
+  (#ait1 #ait2 #ait3 : Type0)
+  (#csch1 : ciview_schema ait1)
+  (#csch2 : ciview_schema ait2)
+  (#csch3 : ciview_schema ait3)
+  (#step12 : aiview_step ait1 ait2)
+  (#step23 : aiview_step ait2 ait3)
   (c1 : ciview_step csch1 csch2 step12)
   (c2 : ciview_step csch2 csch3 step23)
   : ciview_step csch1 csch3 (compose_astep step12 step23) =
@@ -245,7 +229,7 @@ let compose_cstep
 }
 
 val full_view_bij (avw : aiview { is_full_view avw })
-  : Ghost (avw.sch.ait =~ natlt avw.len)
+  : Ghost (avw.ait =~ natlt avw.len)
           (requires True)
           (ensures fun b -> forall x. b.ff x == it_to_nat avw x)
 
@@ -265,7 +249,7 @@ let sum_aiview_fam_len
 type sum_aiview_fam_ait
   (n : pos)
   (vws : natlt n -> aiview)
-  = (i : natlt n & (vws i).sch.ait)
+  = (i : natlt n & (vws i).ait)
 
 let sum_aiview_fam_f
   (n : pos)
@@ -302,9 +286,7 @@ let sum_aiview_fam
   : aiview =
 {
   len = sum_aiview_fam_len n vws;
-  sch = {
-    ait = sum_aiview_fam_ait n vws;
-  };
+  ait = sum_aiview_fam_ait n vws;
   step = {
     imap = {
       f = sum_aiview_fam_f n vws #_;
